examples-c/schorr-waite/coq/BinTree.v
@@ -152,6 +152,8 @@ destruct H.
 apply H0.
 Qed.
 
+
+
 Lemma sans_rep_sublist : forall (l l1 l2 : list pointer), sans_rep l -> 
 l = l1 ++ l2 -> sans_rep l2. 
 induction l.
@@ -170,7 +172,6 @@ rewrite <-app_comm_cons in H0.
 inversion H0.
 auto.
 Qed.
-
 Ltac caseq t := generalize (refl_equal t);pattern t at -1;case t.
 
 
@@ -188,6 +189,52 @@ intros i.
 elim (i H0).
 Qed.
 
+Lemma sans_rep_sublist2 : forall (l l1 l2 : list pointer) ( a : pointer), sans_rep l -> 
+l = l1 ++a::l2 -> sans_rep (l1++l2). 
+induction l.
+intros.
+destruct l1.
+simpl in H0.
+inversion H0.
+inversion H0.
+intros.
+induction l1.
+simpl in *|-*.
+apply sans_rep_sublist1 with a.
+inversion H0;subst.
+auto.
+inversion H0.
+subst.
+unfold sans_rep.
+simpl.
+elim H.
+intros.
+destruct (In_dec eq_pointer_dec a1 (l1 ++ a0::l2) ) .
+inversion H1.
+destruct (In_dec eq_pointer_dec a1 (l1 ++ l2)).
+elim n.
+elim (in_app_or _ _ _ i).
+intro; apply in_or_app; auto.
+intro; apply in_or_app; intuition.
+intuition.
+apply IHl with a0;auto.
+Qed.
+
+Lemma sans_rep_sublist_bis : forall (l2 l l1  : list pointer), sans_rep l -> 
+l = l1 ++ l2 -> sans_rep l1. 
+induction l2.
+intros.
+subst.
+rewrite <- app_nil_end in H.
+auto.
+intros.
+subst.
+assert ((l1 ++ a :: l2) = (l1 ++ a :: l2)).
+auto.
+generalize (sans_rep_sublist2 (l1 ++ a :: l2) l1 l2 a H H0).
+intro.
+apply IHl2 with (l1++l2);auto.
+Qed.
 
 Lemma sans_rep_false : forall (p1 : pointer)(lp : list pointer),
 sans_rep (p1 :: p1 :: lp) -> False.
@@ -200,6 +247,36 @@ apply n.
 left;auto.
 Qed.
 
+Lemma sans_rep_false2 : forall (p1 : pointer)(lp1 lp2 : list pointer),
+sans_rep (p1 ::lp1 ++ p1 :: lp2) -> False.
+intros.
+simpl in H.
+inversion_clear H.
+destruct (In_dec eq_pointer_dec p1 (lp1 ++ p1 :: lp2)).
+inversion H0.
+apply n;clear n.
+clear H1.
+induction lp1.
+simpl;left;auto.
+right;auto.
+Qed.
+
+Lemma sans_rep_p_bis : forall (p1:pointer)(lp1 lp2:list pointer), sans_rep(lp1++p1::lp2)->
+~In p1 lp1.
+intros.
+intro.
+induction lp1.
+inversion H0.
+generalize (eq_pointer_dec a p1).
+intros [p|p].
+subst.
+apply sans_rep_false2 with p1 lp1 lp2;auto.
+apply IHlp1.
+apply sans_rep_sublist1 with a;auto.
+inversion H0.
+elim (p H1).
+auto.
+Qed.
 
 Lemma reachable_no_cycle : forall (a : alloc_table) (p1 p2 : pointer) 
 ( l r : memory pointer) (path : list pointer), reachable a l r p1 p2 (path) -> 
@@ -314,14 +391,6 @@ Definition unmarked_reachable (a: alloc_table) (m:memory Z)
 exists lp : list pointer, (forall x : pointer, In x lp -> (acc m x) = 0 ) 
 /\ reachable a l r p1 p2 lp.
 
-Inductive stkOk   (c:memory Z) (l: memory pointer)(r: memory pointer) 
-(iL : memory pointer)(iR: memory pointer) : pointer ->  list pointer -> Prop :=
-| stkOk_nil : forall t : pointer, stkOk  c l r iL iR t nil 
-| stkOk_cons : forall t : pointer, forall p : pointer, forall stk : list pointer,
-stkOk  c l r iL iR p stk -> ((acc iL p) = if Zneq_bool (acc c p) 0 then (acc l p) else t) -> 
-((acc iR p) = if Zneq_bool (acc c p) 0 then t else (acc r p)) -> 
-stkOk  c l r iL iR t (cons p stk).
-
 Definition clr_list (a: alloc_table)  (c:memory Z) (l: memory pointer)
 (r: memory pointer) : pointer ->list pointer-> Prop :=
 let next t := if Z_eq_dec (acc c t) 0 then (acc l t) else (acc r t) in
@@ -335,3 +404,437 @@ all_in_list m l -> (acc m t) <> 0 -> all_in_list m (cons t l).
 Definition isreachable (a: alloc_table) (l: memory pointer)(r: memory pointer) 
 (p1 :pointer) (p2:pointer) : Prop :=
 exists lp : list pointer, reachable a l r p1 p2 lp. 
+
+(* WF relation over graph *)
+
+Record var_type : Set := mkvar_type
+  { a : alloc_table;
+    m : memory Z;
+    c : memory Z;
+     l : memory pointer;
+     r : memory pointer;
+     p : pointer;
+     t : pointer
+    }.
+
+Definition reachable_elements (a:alloc_table) (l r:memory pointer) (p t: pointer)
+(lp : list pointer):Prop :=
+sans_rep lp/\
+forall p2 : pointer ,p2<> null-> (isreachable a l r p p2 \/isreachable a l r t p2) <-> In p2 lp.
+
+Fixpoint mesure_mark (m : memory Z) (l : list pointer) {struct l} : nat :=
+match l with
+| nil => 0%nat
+| p::l => plus ( if Z_eq_dec (acc m p) 0 then 1%nat else 0%nat) (mesure_mark m l)
+end.
+
+Lemma mesure_mark_a : forall m : memory Z , forall lp1a lp1b : list pointer,
+(plus (mesure_mark m lp1a) (mesure_mark m lp1b))  = mesure_mark m (lp1a++lp1b).
+intros.
+induction lp1a.
+simpl;auto.
+case (Z_eq_dec (acc m0 a0) 0).
+simpl.
+intros.
+replace (acc m0 a0) with 0;auto.
+simpl.
+apply (f_equal S).
+auto.
+simpl.
+intros.
+intuition.
+Qed.
+
+Lemma mesure_mark_b : forall p : pointer , forall lp1 lp2a lp2b : list pointer ,
+sans_rep (p::lp1)-> sans_rep (lp2a++p::lp2b)->
+(forall q : pointer , In q (p::lp1) -> In q (lp2a++p::lp2b)) ->
+(forall q : pointer, In q lp1 -> In q (lp2a ++ lp2b)).
+intros.
+case (eq_pointer_dec q p0).
+intro.
+subst.
+generalize  (sans_rep_p p0 lp1 H).
+intuition.
+intro.
+assert (In q (lp2a ++ p0 :: lp2b) -> In q (lp2a++lp2b)).
+intros.
+apply in_or_app.
+generalize (in_app_or lp2a (p0::lp2b) q H3) .
+intros [H4|H4].
+left;auto.
+destruct H4.
+elim (n );auto.
+right;auto.
+apply H3.
+apply H1.
+right;auto.
+Qed.
+
+Lemma sans_rep_sublist3 : forall (l l1 l2 : list pointer) ( a : pointer), sans_rep l -> 
+l = l1 ++a::l2 -> sans_rep (a::l1++l2). 
+induction l0.
+intros.
+destruct l1.
+simpl in H0.
+inversion H0.
+inversion H0.
+intros.
+destruct l1.
+simpl in *|-*.
+inversion H.
+inversion H0;subst;auto.
+inversion H0;subst.
+rewrite <- app_comm_cons.
+inversion H.
+case (In_dec eq_pointer_dec p0 (a1 :: l1 ++ l2));intros.
+destruct (In_dec eq_pointer_dec p0 (l1 ++ a1 :: l2));intros.
+inversion H1.
+elim n.
+apply in_or_app.
+rewrite app_comm_cons in i.
+generalize (in_app_or (a1:: l1) l2 p0 i).
+intuition.
+generalize (in_inv H4).
+intuition.
+right;left;auto.
+rewrite <- app_comm_cons in H0.
+assert (l1 ++ a1 :: l2 = l1 ++ a1 :: l2).
+auto.
+generalize (IHl0 l1 l2 a1 H2 H3).
+intro.
+simpl.
+case (In_dec eq_pointer_dec a1 (p0 :: l1 ++ l2));intro.
+inversion i.
+subst.
+elim n.
+left;auto.
+inversion H4.
+destruct (In_dec eq_pointer_dec a1 (l1 ++ l2)).
+inversion H6.
+elim (n0 H5).
+split;auto.
+split.
+destruct (In_dec eq_pointer_dec p0 (l1 ++ l2)).
+elim n.
+right;auto.
+auto.
+apply sans_rep_sublist1 with a1;auto.
+Qed.
+
+Lemma mesure_mark_c : forall p : pointer , forall lp1 lp2a lp2b : list pointer ,
+sans_rep (p::lp1)-> sans_rep (lp2a++p::lp2b)->
+(forall q : pointer ,  In q (lp2a++p::lp2b)->In q (p::lp1) ) ->
+(forall q : pointer,  In q (lp2a ++ lp2b)->In q lp1 ).
+intros.
+case (eq_pointer_dec q p0).
+intro.
+subst.
+assert (lp2a ++ p0 :: lp2b = lp2a ++ p0 :: lp2b).
+auto.
+generalize (sans_rep_sublist2 (lp2a ++ p0 :: lp2b) lp2a lp2b p0 H0 H3);intro.
+generalize (sans_rep_sublist (lp2a++p0::lp2b) lp2a (p0::lp2b)  H0).
+intros.
+generalize (sans_rep_sublist3 (lp2a ++ p0 :: lp2b) lp2a lp2b p0 H0 H3).
+intro.
+inversion H6.
+destruct (In_dec eq_pointer_dec p0 (lp2a ++ lp2b)).
+inversion H7.
+elim ( n H2).
+intro.
+assert (In q (lp2a ++ p0 :: lp2b)).
+generalize ( in_app_or lp2a lp2b q H2).
+intuition.
+generalize (H1 q H3);intro.
+inversion H4.
+elim (n ).
+auto.
+auto.
+Qed.
+
+Lemma mesure_mark_bbis : forall (l1 l2 : list pointer) ( m : memory Z), 
+mesure_mark m (l1++l2) = plus (mesure_mark m l1) (mesure_mark m l2).
+intros.
+induction l1.
+simpl;auto.
+simpl.
+destruct (Z_eq_dec (acc m0 a0) 0).
+replace (acc m0 a0) with 0;auto.
+simpl.
+apply (f_equal S).
+auto.
+simpl.
+auto.
+Qed.
+
+
+Lemma mesure_mark_bis : forall m : memory Z,forall lp1 lp2 : list pointer , (forall p : pointer, 
+In p lp1 -> In p lp2)-> (forall p : pointer, In p lp2 -> In p lp1) ->sans_rep lp1 -> sans_rep lp2->mesure_mark m lp1 = mesure_mark m lp2.
+intros m0 lp1.
+induction lp1.
+destruct lp2.
+auto.
+assert (In p0 (p0::lp2)).
+left;auto.
+intros.
+elim (H1 p0 H).
+assert ( In a0 (a0::lp1)).
+left;auto.
+intros.
+generalize (H0 a0 H).
+intro.
+generalize (split_list a0 lp2 H4). 
+intros (lp2a,(lp2b,sub)).
+subst.
+generalize ( mesure_mark_a m0 lp2a (a0::lp2b)).
+intro.
+replace (mesure_mark m0 (lp2a ++ a0 :: lp2b)) with (mesure_mark m0 lp2a + mesure_mark m0 (a0 :: lp2b))%nat;auto.
+assert (mesure_mark m0 lp1 = mesure_mark m0 (lp2a++lp2b)).
+apply IHlp1.
+apply mesure_mark_b with a0;auto .
+apply mesure_mark_c with a0;auto .
+apply sans_rep_sublist1 with a0;auto.
+apply (sans_rep_sublist2 (lp2a ++ a0 :: lp2b) lp2a lp2b a0 H3) .
+auto.
+simpl.
+destruct (Z_eq_dec (acc m0 a0)).
+simpl.
+rewrite <- plus_n_Sm.
+rewrite H6.
+apply (f_equal S).
+apply mesure_mark_bbis.
+simpl.
+rewrite H6.
+apply mesure_mark_bbis.
+Qed.
+
+Lemma reacha_element : forall (a:alloc_table) (l r:memory pointer) (p t: pointer) (m : memory Z),
+  forall lp1 lp2,reachable_elements a l r p t lp1 /\ reachable_elements a l r p t lp2 ->
+  (forall (q : pointer) , In q lp1 <-> In q lp2).
+intuition;inversion_clear H0;inversion_clear H1;generalize (H3 q);generalize (H4 q);
+intuition.
+Qed.
+
+
+Lemma mesure_mark_function : 
+  forall (a:alloc_table) (l r:memory pointer) (p t: pointer) (m : memory Z),
+  forall lp1 lp2,
+reachable_elements a l r p t lp1 /\ reachable_elements a l r p t lp2
+-> mesure_mark (m : memory Z) lp1 = mesure_mark (m : memory Z) lp2.
+intros.
+generalize (reacha_element a0 l0 r0 p0 t0 m0 lp1 lp2 H).
+intro.
+apply mesure_mark_bis;intros.
+generalize (H0 p1);intuition.
+generalize (H0 p1);intuition.
+inversion_clear H.
+inversion H1;auto.
+inversion_clear H.
+inversion H2;auto.
+Qed.
+
+Definition order_mark_m  (e1 e2 : var_type): Prop :=
+exists lp1 : list pointer,
+  exists lp2 : list pointer,
+    reachable_elements e1.(a) e1.(l) e1.(r) e1.(p) e1.(t) lp1 /\ 
+    reachable_elements e2.(a) e2.(l) e2.(r) e2.(p) e2.(t) lp2 /\
+lt (mesure_mark e1.(m) lp1)  (mesure_mark e2.(m) lp2).
+
+Definition order_mark_c  (e1 e2 : var_type): Prop :=
+exists lp1 : list pointer,
+  exists lp2 : list pointer,
+    reachable_elements e1.(a) e1.(l) e1.(r) e1.(p) e1.(t) lp1 /\ 
+    reachable_elements e2.(a) e2.(l) e2.(r) e2.(p) e2.(t) lp2 /\ 
+lt (mesure_mark e1.(c) lp1)  (mesure_mark e2.(c) lp2).
+
+Definition order_pile (e1 e2 : var_type) : Prop :=
+exists pile1 : list pointer,
+    exists pile2 : list pointer,
+      clr_list e1.(a) e1.(c) e1.(l) e1.(r) e1.(p) pile1 /\ 
+      clr_list e2.(a) e2.(c) e2.(l) e2.(r) e2.(p) pile2 /\ 
+       lt (List.length pile1)  (List.length pile2).
+
+Require Export Lexicographic_Product.
+Require Import Relation_Operators.
+
+
+Lemma order_mark_m_wf : well_founded order_mark_m.
+Proof.
+apply well_founded_inv_lt_rel_compat with (fun (e1:var_type) (n : nat) 
+=>
+exists lp1 : list pointer ,
+    reachable_elements e1.(a) e1.(l) e1.(r) e1.(p) e1.(t) lp1 /\
+    n = mesure_mark e1.(m) lp1).
+unfold order_mark_m,inv_lt_rel.
+intros x y (pile1,(pile2,H)).
+exists (mesure_mark (m x) pile1).
+exists pile1.
+intuition.
+intro.
+intros (pile3,(H1,H2)).
+intuition.
+subst m0.
+assert ((mesure_mark (m y) pile3) = (mesure_mark (m y) pile2)).
+apply (mesure_mark_function (a y) (l y) (r y) (p y) (t y) (m y) pile3 pile2).
+split;auto.
+rewrite H2.
+auto.
+Qed.
+
+Lemma order_mark_c_wf : well_founded order_mark_c.
+Proof.
+apply well_founded_inv_lt_rel_compat with (fun (e1:var_type) (n : nat) 
+=>
+exists lp1 : list pointer ,
+    reachable_elements e1.(a) e1.(l) e1.(r) e1.(p) e1.(t) lp1 /\
+    n = mesure_mark e1.(c) lp1).
+unfold order_mark_c,inv_lt_rel.
+intros x y (pile1,(pile2,H)).
+exists (mesure_mark (c x) pile1).
+exists pile1.
+intuition.
+intro.
+intros (pile3,(H1,H2)).
+intuition.
+subst m0.
+assert ((mesure_mark (c y) pile3) = (mesure_mark (c y) pile2)).
+apply (mesure_mark_function (a y) (l y) (r y) (p y) (t y) (c y) pile3 pile2).
+split;auto.
+rewrite H2.
+auto.
+Qed.
+
+(*
+Lemma order_pile_wf : well_founded order_pile.
+Proof.
+apply well_founded_inv_lt_rel_compat with (fun (e1:var_type) (n : nat) 
+=>
+exists pile1 : list pointer ,
+(clr_list e1.(a) e1.(c) e1.(l) e1.(r) e1.(p) pile1 /\ n=(List.length pile1))).
+unfold order_pile,inv_lt_rel.
+intros x y (pile1,(pile2,H)).
+exists (List.length pile1).
+exists pile1.
+intuition.
+intro.
+intros (pile3,(H1,H2)).
+intuition.
+subst m0.
+replace pile3 with pile2;intuition .
+Print clr_list.
+apply llist_function with (next :=(fun t : pointer => if Z_eq_dec (acc (c y) t) 0 then acc (l y) t else acc (r y) t))
+( a := (a y)) (a' := (a y)) (p:= (p y));trivial.
+Qed.
+*)
+
+Section lexico.
+
+Variables A B : Set.
+
+Variable Ra : A -> A -> Prop.
+Variable Rb : B -> B -> Prop.
+
+Definition lex := lexprod A (fun _:A => B) Ra (fun _:A => Rb).
+
+Lemma lex_well_founded :
+ well_founded Ra -> well_founded Rb -> well_founded lex.
+Proof.
+intros wfa wfb.
+exact
+ (wf_lexprod A (fun _:A => B) Ra (fun _:A => Rb) wfa (fun _ => wfb)).
+Qed.
+
+End lexico.
+
+Section LT_WF_REL.
+Variable A : Set.
+
+Variable X : Set.
+Variable lt : X -> X -> Prop.
+Variable F : A -> X -> Prop.
+Definition inv_lt_rel x y :=
+   exists2 n : _, F x n & (forall m, F y m -> lt n m).
+
+Hypothesis lt_wf : well_founded lt.
+
+Remark acc_lt_rel : forall x:A, (exists n : _, F x n) -> Acc inv_lt_rel x.
+intros x [n fxn]; generalize x fxn; clear x fxn.
+pattern n; apply (well_founded_induction_type lt_wf); intros.
+constructor; intros.
+inversion H0.
+apply (H x1); auto.
+Qed.
+
+Theorem well_founded_inv_rel_compat : well_founded inv_lt_rel.
+constructor; intros.
+inversion H.
+apply acc_lt_rel; trivial.
+exists x; trivial.
+Qed.
+
+End LT_WF_REL.
+
+Definition lex_nat := lex _ _ lt lt.
+
+Lemma lex_nat_well_founded : well_founded lex_nat.
+exact (lex_well_founded _ _ lt lt lt_wf lt_wf).
+Qed.
+
+Definition interp_mark_m  (e : var_type) (n:nat): Prop :=
+exists lp : list pointer,
+    reachable_elements e.(a) e.(l) e.(r) e.(p) e.(t) lp /\ 
+  (mesure_mark e.(m) lp)=n.
+
+Definition interp_mark_c  (e: var_type) (n:nat): Prop :=
+exists lp : list pointer,
+    reachable_elements e.(a) e.(l) e.(r) e.(p) e.(t) lp /\ 
+   (mesure_mark e.(c) lp)=n.
+
+Definition interp_pile (e : var_type) (n:nat) : Prop :=
+exists pile : list pointer,
+      clr_list e.(a) e.(c) e.(l) e.(r) e.(p) pile /\ 
+       (List.length pile)=n.
+
+Definition natnat := {x : nat & nat}.
+
+Definition interp_mark_c_and_stack (e : var_type) (p: natnat) : Prop :=
+  let (n,m) := p in
+    interp_mark_c e n /\ interp_pile e m.
+
+Definition order_mark_c_and_stack : var_type -> var_type -> Prop := 
+  inv_lt_rel var_type natnat lex_nat interp_mark_c_and_stack.
+
+Lemma order_mark_c_and_stack_wf : 
+  well_founded order_mark_c_and_stack.
+Proof.
+unfold order_mark_c_and_stack.
+apply well_founded_inv_rel_compat.
+apply lex_nat_well_founded.
+Qed.
+
+Definition natnatnat := {x : nat & natnat}.
+
+Definition interp_mark_m_and_c_and_stack (e : var_type) (t: natnatnat) : Prop :=
+  let (n,p) := t in
+    interp_mark_m e n /\ interp_mark_c_and_stack e p.
+
+Definition lex_natnatnat := lex _ _ lt lex_nat.
+
+Lemma lex_natnatnat_well_founded : well_founded lex_natnatnat.
+exact (lex_well_founded _ _ lt lex_nat lt_wf lex_nat_well_founded).
+Qed.
+
+Definition order_mark_m_and_c_and_stack : var_type -> var_type -> Prop := 
+  inv_lt_rel var_type natnatnat lex_natnatnat interp_mark_m_and_c_and_stack.
+
+
+Lemma order_mark_m_and_c_and_stack_wf : 
+  well_founded order_mark_m_and_c_and_stack.
+Proof.
+unfold order_mark_m_and_c_and_stack.
+apply well_founded_inv_rel_compat.
+apply lex_natnatnat_well_founded.
+Qed.
+
+
+
+
